(A3) $(x+y)+z=(a+c,\,b+d)+(e,f)$

$=(a+c+e,\,b+d+f)$

$=(a,\,b)+(c+e,\,d+f)=x+(y+z)$.

(A4) $x+0=(a,\,b)+(0,\,0)=(a,\,b)=x$.

(A5) Put $-x=(-a,\,-b)$. Then $x+(-x)=(0,\,0)=0$.

(M1) is clear.

(M2) $xy=(ac-bd,\,ad+bc)=(ca-db,\,da+cb)=yx$.

(M3) $(xy)z=(ac-bd,\,ad+bc)(e,f)$

$=(ace-bde-adf-bcf,\,aef-bdf+ade+bce)$

$=(a,\,b)(ce-df,\,cf+de)=x(yz)$.

(M4) $1x=(1,\,0)(a,\,b)=(a,\,b)=x$.

(M5) If $x\neq 0$ then $(a,\,b)\neq(0,\,0)$, which means that at least one of the real numbers $a$, $b$ is different from $0$. Hence $a^{2}+b^{2}>0$, by Proposition 1.18$(d)$, and we can define

$$\frac{1}{x}=\left(\frac{a}{a^{2}+b^{2}},\,\,\,\,\frac{-b}{a^{2}+b^{2}}\right).$$

Then

$$x\cdot\frac{1}{x}=(a,\,b)\left(\frac{a}{a^{2}+b^{2}},\,\,\,\,\frac{-b}{a^{2}+b ^{2}}\right)=(1,\,0)=1.$$

(D) $x(y+z)=(a,\,b)(c+e,\,d+f)$

$=(ac+ae-bd-bf,\,ad+af+bc+be)$

$=(ac-bd,\,ad+bc)+(ae-bf,\,af+be)$

$=xy+xz$.

**1.26**: _For any real numbers $a$ and $b$ we have_

$$(a,\,0)+(b,\,0)=(a+b,\,0),\,\,\,\,\,\,\,\,\,\,(a,\,0)(b,\,0)=(ab,\,0).$$

The proof is trivial.

Theorem 1.26 shows that the complex numbers of the form $(a,\,0)$ have the same arithmetic properties as the corresponding real numbers $a$. We can therefore identify $(a,\,0)$ with $a$. This identification gives us the real field as a subfield of the complex field.

The reader may have noticed that we have defined the complex numbers without any reference to the mysterious square root of $-1$. We now show that the notation $(a,\,b)$ is equivalent to the more customary $a+bi$.

**1.27**: _Definition_ $i=(0,\,1)$._