**Proof** ($a$) and ($b$) are trivial. Put $z=a+bi$, $w=c+di$, with $a$, $b$, $c$, $d$ real. Then

$$|zw|^{2}=(ac-bd)^{2}+(ad+bc)^{2}=(a^{2}+b^{2})(c^{2}+d^{2})=|z|^{2}|w|^{2}$$

or $|zw|^{2}=(|z|\,|w|)^{2}$. Now ($c$) follows from the uniqueness assertion of Theorem 1.21.

To prove ($d$), note that $a^{2}\leq a^{2}+b^{2}$, hence

$$|a|=\sqrt{a^{2}}\leq\sqrt{a^{2}+b^{2}}.$$

To prove ($e$), note that $\bar{z}w$ is the conjugate of $z\bar{w}$, so that $z\bar{w}+\bar{z}w=2\ \mathrm{Re}\ (z\bar{w})$. Hence

$$|z+w|^{2} =(z+w)(\bar{z}+\bar{w})=z\bar{z}+z\bar{w}+\bar{z}w+w\bar{w}$$ $$=|z|^{2}+2\ \mathrm{Re}\ (z\bar{w})+|w|^{2}$$ $$\leq|z|^{2}+2\,|z\bar{w}|\,+\,|w|^{2}$$ $$=|z|^{2}+2\,|z|\,|w|\,+\,|w|^{2}=(|z|\,+\,|w|)^{2}.$$

Now ($e$) follows by taking square roots.

### Notation

If $x_{1}$,..., $x_{n}$ are complex numbers, we write

$$x_{1}+x_{2}+\cdots+x_{n}=\sum_{j=1}^{n}x_{j}\,.$$

We conclude this section with an important inequality, usually known as the _Schwarz inequality_.

**1.35**: **Theorem** _If $a_{1}$,..., $a_{n}$ and $b_{1}$,..., $b_{n}$ are complex numbers, then_

$$\left|\,\sum_{j=1}^{n}a_{j}\,\bar{b}_{j}\,\right|^{2}\leq\sum_{j=1}^{n}|a_{j}| ^{\,2}\sum_{j=1}^{n}|b_{j}|^{\,2}.$$

**Proof** Put $A=\Sigma\,|a_{j}|^{\,2}$, $B=\Sigma\,|\,b_{j}|^{\,2}$, $C=\Sigma a_{j}\,\bar{b}_{j}$ (in all sums in this proof, $j$ runs over the values $1$,..., $n$). If $B=0$, then $b_{1}=\cdots=b_{n}=0$, and the conclusion is trivial. Assume therefore that $B>0$. By Theorem 1.31 we have

$$\sum\,|Ba_{j}-Cb_{j}|^{\,2} =\sum\,(Ba_{j}-Cb_{j})(B\bar{a}_{j}-\overline{Cb_{j}})$$ $$=B^{2}\sum\,|a_{j}|^{\,2}-B\overline{C}\sum\,a_{j}\,\bar{b}_{j}- BC\sum\,\bar{a}_{j}\,b_{j}+|C|^{\,2}\sum\,|b_{j}|^{\,2}$$ $$=B^{2}A-B|\,C|^{\,2}$$ $$=B(AB-|\,C|^{\,2}).$$