Since each term in the first sum is nonnegative, we see that

$$B(AB-\mid C\mid^{2})\geq 0.$$

Since $B>0$, it follows that $AB-\mid C\mid^{2}\geq 0$. This is the desired inequality.

Euclidean Spaces

DefinitionsFor each positive integer $k$, let $R^{k}$ be the set of all ordered $k$-tuples

$$\mathbf{x}=(x_{1},\,x_{2}\,,\,\ldots,\,x_{k}),$$

where $x_{1}$,..., $x_{k}$ are real numbers, called the _coordinates_ of $\mathbf{x}$. The elements of $R^{k}$ are called points, or vectors, especially when $k>1$. We shall denote vectors by boldfaced letters. If $\mathbf{y}=(y_{1},\,\ldots,\,y_{k})$ and if $\alpha$ is a real number, put

$$\mathbf{x}+\mathbf{y} =(x_{1}+y_{1},\,\ldots,\,x_{k}+y_{k}),$$ $$\alpha\mathbf{x} =(\alpha x_{1},\,\ldots,\,\alpha x_{k})$$

so that $\mathbf{x}+\mathbf{y}\in R^{k}$ and $\alpha\mathbf{x}\in R^{k}$. This defines addition of vectors, as well as multiplication of a vector by a real number (a scalar). These two operations satisfy the commutative, associative, and distributive laws (the proof is trivial, in view of the analogous laws for the real numbers) and make $R^{k}$ into a _vector space over the real field_. The zero element of $R^{k}$ (sometimes called the _origin_ or the _null vector_) is the point $\mathbf{0}$, all of whose coordinates are $0$.

We also define the so-called "inner product" (or scalar product) of $\mathbf{x}$ and $\mathbf{y}$ by

$$\mathbf{x}\cdot\mathbf{y}=\sum_{i=1}^{k}x_{i}y_{i}$$

and the _norm_ of $\mathbf{x}$ by

$$\mid\mathbf{x}\mid\,=(\mathbf{x}\cdot\mathbf{x})^{1/2}=\left(\sum_{1}^{k}x_{i }^{2}\right)^{1/2}.$$

The structure now defined (the vector space $R^{k}$ with the above inner product and norm) is called euclidean $k$-space.

**Theorem** : _Suppose $\mathbf{x}$, $\mathbf{y}$, $\mathbf{z}\in R^{k}$, and $\alpha$ is real. Then_

$$\begin{array}{ll}(a)&\mid\mathbf{x}\mid\,\geq 0;\\ (b)&\mid\mathbf{x}\mid\,=0\text{ if and only if }\mathbf{x}=\mathbf{0}\,;\\ (c)&\mid\alpha\mathbf{x}\mid\,=\,\mid\mathbf{x}\,\mid\,\mathbf{x}\,\mid;\\ (d)&\mid\mathbf{x}\cdot\mathbf{y}\mid\,\leq\,\mid\mathbf{x}\,\mid\,\mathbf{y} \,\mid;\\ (e)&\mid\mathbf{x}+\mathbf{y}\mid\,\leq\,\mid\mathbf{x}\,\mid\,+\,\mid \mathbf{y}\,\mid;\\ (f)&\mid\mathbf{x}-\mathbf{z}\mid\,\leq\,\mid\mathbf{x}-\mathbf{y}\,\mid\,+\, \mid\mathbf{y}-\mathbf{z}\,\mid.\end{array}$$