### The distributive law

$$x(y+z)=xy+xz$$

holds for all $x$, $y$, $z\in F$.

### Remarks

1. One usually writes (in any field) $$x-y,\frac{x}{y},x+y+z,xyz,x^{2},x^{3},2x,3x,\ldots.$$ in place of $$x+(-y),x\cdot\left(\frac{1}{y}\right),(x+y)+z,(xy)z,xx,xxx,x+x,x+x+x,\ldots.$$ 2. The field axioms clearly hold in $Q$, the set of all rational numbers, if addition and multiplication have their customary meaning. Thus $Q$ is a field.
3. Although it is not our purpose to study fields (or any other algebraic structures) in detail, it is worthwhile to prove that some familiar properties of $Q$ are consequences of the field axioms; once we do this, we will not need to do it again for the real numbers and for the complex numbers.

### Proposition

_The axioms for addition imply the following statements._

1. _If_ $x+y=x+z$ _then_ $y=z$_._
2. _If_ $x+y=x$ _then_ $y=0$_._
3. _If_ $x+y=0$ _then_ $y=-x$_._
4. $-(-x)=x$_._

Statement ($a$) is a cancellation law. Note that ($b$) asserts the uniqueness of the element whose existence is assumed in (A4), and that ($c$) does the same for (A5).

**Proof** If $x+y=x+z$, the axioms (A) give

$$\begin{array}{l}y=0+y=(-x+x)+y=-x+(x+y)\\ =-x+(x+z)=(-x+x)+z=0+z=z.\end{array}$$ This proves ($a$). Take $z=0$ in ($a$) to obtain ($b$). Take $z=-x$ in ($a$) to obtain ($c$).

Since $-x+x=0$, ($c$) (with $-x$ in place of $x$) gives ($d$).