**1.15**: **Proposition** _The axioms for multiplication imply the following statements._

1. _If_ $x\neq 0$ _and_ $xy=xz$ _then_ $y=z$_._
2. _If_ $x\neq 0$ _and_ $xy=x$ _then_ $y=1$_._
3. _If_ $x\neq 0$ _and_ $xy=1$ _then_ $y=1/x$_._
4. _If_ $x\neq 0$ _then_ $1/(1/x)=x$_._

The proof is so similar to that of Proposition 1.14 that we omit it.

**1.16**: **Proposition** _The field axioms imply the following statements, for any $x$, $y$, $z\in F$._

1. $0x=0$_._
2. _If_ $x\neq 0$ _and_ $y\neq 0$ _then_ $xy\neq 0$_._
3. $(-x)y=-(xy)=x(-y)$_._
4. $(-x)(-y)=xy$_._

**Proof**$0x+0x=(0+0)x=0x$. Hence $1.14(b)$ implies that $0x=0$, and $(a)$ holds.

Next, assume $x\neq 0$, $y\neq 0$, but $xy=0$. Then $(a)$ gives

$$1=\begin{pmatrix}1\\ -y\end{pmatrix}\begin{pmatrix}1\\ x\end{pmatrix}xy=\begin{pmatrix}1\\ y\end{pmatrix}\begin{pmatrix}1\\ x\end{pmatrix}0=0,$$

a contradiction. Thus $(b)$ holds.

The first equality in $(c)$ comes from

$$(-x)y+xy=(-x+x)y=0y=0,$$

combined with $1.14(c)$; the other half of $(c)$ is proved in the same way. Finally,

$$(-x)(-y)=-[x(-y)]=-[-(xy)]=xy$$

by $(c)$ and $1.14(d)$.

**1.17**: **Definition** An _ordered field_ is a _field_$F$ which is also an _ordered set_, such that

1. $x+y<x+z$ if $x$, $y$, $z\in F$ and $y<z$,
2. $xy>0$ if $x\in F$, $y\in F$, $x>0$, and $y>0$.

If $x>0$, we call $x$_positive_; if $x<0$, $x$ is _negative_.

For example, $Q$ is an ordered field.

All the familiar rules for working with inequalities apply in every ordered field: Multiplication by positive [negative] quantities preserves [reverses] inequalities, no square is negative, etc. The following proposition lists some of these.